Put state_error

theories/Semantics.v
@@ -5,12 +5,12 @@ Inductive sort: Type :=
 | angelic
 | demonic
 | final
+| error
 .
 
 Record semantics : Type := Semantics_gen {
   state: Type;
   step : state -> option event -> state -> Prop;
   initial_state: state;
-  (* final_state: state -> Prop; *)
   state_sort: state -> sort;
 }.
